move definition of initial game to AKE_proof (simpler to diff games if all games are in one file)

examples/AKE/AKE_proof.ec
@@ -7,15 +7,254 @@ require import Fun.
 require import Real.
 
 require import AKE_defs.
-require import AKE_g0.
+
+(*{ Initial game and security definition *)
+
+(* The initial module: we keep it simple and inline the
+   definitions of h1 and h2. *)
+module AKE(FA : Adv) = {
+  
+  var evs  : Event list               (* events for queries performed by adversary *)
+  var test : Sid option               (* session id of test session *)
+
+  var cSession, cH1, cH2 : int        (* counters for queries *)
+
+  var mH1 : ((Sk * Esk), Eexp) map    (* map for h1 *)
+  var sH1 : (Sk * Esk) set            (* adversary queries for h1 *)
+
+  var mH2 : (Sstring, Key) map        (* map for h2 *)
+  var sH2 : Sstring set               (* adversary queries for h2 *)
+
+  var mSk        : (Agent, Sk) map    (* map for static secret keys *)
+  var mStarted   : (Sidx, Sdata) map  (* map of started sessions *)
+  var mCompleted : (Sidx, Epk)   map  (* additional data for completed sessions *)
+  
+  module O : AKE_Oracles = {
+
+    fun h1(a : Sk, x : Esk) : Eexp = {
+      var e : Eexp;
+      e = $sample_Eexp;
+      if (!in_dom (a,x) mH1) {
+        cH1 = cH1 + 1;
+        mH1.[(a,x)] = e;
+      } 
+      return proj mH1.[(a,x)];
+    }
+
+    fun h1_a(a : Sk, x : Esk) : Eexp option = {
+      var r : Eexp option = None;
+      var xe : Eexp;
+      if (cH1 < qH1) {
+        cH1 = cH1 + 1;
+        sH1 = add (a,x) sH1;
+        xe = h1(a,x);
+        r = Some(xe);
+      }
+      return r;
+    }
+
+    fun h2(sstring : Sstring) : Key = {
+      var ke : Key;
+      ke = $sample_Key;
+      if (!in_dom sstring mH2) {
+        mH2.[sstring] = ke;
+      }
+      return proj mH2.[sstring];
+    }
+ 
+    fun h2_a(sstring : Sstring) : Key option = {
+      var r : Key option = None;
+      var ks : Key;
+      if (cH2 < qH2) {
+        cH2 = cH2 + 1;
+        sH2 = add sstring sH2;
+        ks = h2(sstring);
+        r = Some(ks);
+      }
+      return r;
+    }
+
+    fun init1(i : Sidx, A : Agent, B : Agent) : Epk option = {
+      var x : Esk;
+      var x' : Eexp;
+      var pX : Epk;
+      var r : Epk option = None; 
+      if (cSession < qSession && in_dom A mSk && in_dom B mSk && !in_dom i mStarted) {
+        cSession = cSession + 1;
+        x  = $sample_Esk;
+        x' = h1(proj (mSk.[A]),x);
+        pX = gen_epk(x');
+        mStarted.[i] = (A,B,x,x',init);
+        r = Some(pX);
+        evs = Start(psid_of_sdata(proj mStarted.[i]))::evs;
+      }
+      return r;
+    }
+
+    fun resp(i : Sidx, B : Agent, A : Agent, X : Epk) : Epk option = {
+      var y : Esk;
+      var y' : Eexp;
+      var pY : Epk;
+      var r : Epk option = None; 
+      if (   cSession < qSession && in_dom A mSk && in_dom B mSk
+          && !in_dom i mStarted && !in_dom i mCompleted) {
+        cSession = cSession + 1;
+        y  = $sample_Esk;
+        y' = h1(proj (mSk.[B]),y);
+        pY = gen_epk(y');
+        mStarted.[i] = (B,A,y,y',resp);
+        mCompleted.[i] = X;
+        r = Some(pY);
+        evs = Accept(sid_of_sdata (proj mStarted.[i]) X)::evs;
+      }
+      return r;
+    }
+
+    fun init2(i : Sidx, Y : Epk) : unit = {
+      if (!in_dom i mCompleted && in_dom i mStarted) {
+        mCompleted.[i] = Y;
+        evs = Accept(sid_of_sdata(proj mStarted.[i]) Y)::evs;
+      }
+    }
+
+    fun staticRev(A : Agent) : Sk option = {
+      var r : Sk option = None;
+      if (in_dom A mSk) {
+        r = mSk.[A];
+        evs = StaticRev(A)::evs;
+      }
+      return r;
+    }
+
+    fun ephemeralRev(i : Sidx) : Esk option = {
+      var r : Esk option = None;
+      if (in_dom i mStarted) {
+        r = Some(sd_esk(proj mStarted.[i]));
+        evs = EphemeralRev(psid_of_sdata(proj mStarted.[i]))::evs;
+      }
+      return r;
+    }
+
+    fun computeKey(i : Sidx) : Key option = {
+      var rv : Key option = None;
+      var a, b : Agent;
+      var r : Role;
+      var x' : Eexp;
+      var x : Esk;
+      var key : Key;
+      if (in_dom i mCompleted) {
+        (a,b,x,x',r) = proj mStarted.[i];
+        key = h2(gen_sstring x' (proj mSk.[a]) b (proj mCompleted.[i]) r);
+        rv = Some key;
+      }
+      return rv;
+    }
+
+    fun sessionRev(i : Sidx) : Key option = {
+      var r : Key option = None;
+      var s : Sid;
+      if (in_dom i mCompleted) {
+        s = sid_of_sdata (proj mStarted.[i]) (proj mCompleted.[i]);
+        evs = SessionRev(sid_of_sdata(proj mStarted.[i]) (proj mCompleted.[i]))::evs;
+        r = computeKey(i);
+      }
+      return r;
+    }
+  }
+  
+  module A = FA(O)
+
+  fun main() : bool = {
+    var b : bool;
+    var pks : Pk list = [];
+    var t_idx : Sidx;
+    var key : Key;
+    var keyo : Key option;
+    var b' : bool = false;
+    var i : int = 0;
+    var ska : Sk;
+    var pka : Pk;
+
+    mSk = Map.empty;
+    while (i < qAgent) {
+      ska = $sample_Sk;
+      pka = gen_pk(ska);
+      pks = pka :: pks;
+      mSk.[pka] = ska;
+    } 
+    cSession = 0;
+    cH1 = 0;
+    cH2 = 0;
+    mH1 = Map.empty;
+    sH1 = FSet.empty;
+    mH2 = Map.empty;
+    sH2 = FSet.empty;
+    mStarted = Map.empty;
+    mCompleted = Map.empty;
+    evs = [];
+    test = None;
+
+    t_idx = A.choose(pks);
+    b = ${0,1};
+    if (mStarted.[t_idx] <> None && mCompleted.[t_idx] <> None) {
+      test = Some (sid_of_sdata (proj mStarted.[t_idx]) (proj mCompleted.[t_idx]));
+        (* the if-condition implies "mem (Accept (proj O.test)) O.evs" *)
+      if (b) {
+        keyo = O.computeKey(t_idx);
+      } else {
+        key  = $sample_Key;
+        keyo = Some key;
+      }
+      b' = A.guess(keyo);
+    }
+    return (b = b');
+  }
+}.
+
 
 pred test_fresh(t : Sid option, evs : Event list) =
   t <> None /\ fresh (proj t) evs.
 
-(* For some small eps to be determined later, we want to prove *)
-const eps : real.
+(*{ Explain security notion *)
+section.
+  (* For an arbitrary adversary A, *)
+  declare module A : Adv.
 
-lemma Secure:
-  forall (A <: Adv) &m,
-    2%r * Pr[   AKE(A).main() @ &m : res /\ test_fresh AKE.test AKE.evs] - 1%r < eps
-by admit.
+  (* we want to a find (small) bound eps *)
+  const eps : real.
+
+  (* such that the advantage of the adversary is upper bounded by eps. *)
+  axiom Secure:
+    forall &m,
+      2%r * Pr[   AKE(A).main() @ &m : res /\ test_fresh AKE.test AKE.evs] - 1%r < eps.
+end section.
+(*} end: Explain security notion *)
+
+(*} end: Initial game and security definition *)
+
+lemma Eq_G0_G0_1_1:
+  forall (A <: Adv),
+    equiv[  AKE(A).main ~ G0_1_0(A).main
+          : true ==> ={res} /\ (test_fresh AKE.test AKE.evs){1} = 
+                               (test_fresh G0_1_0.test G0_1_0.evs){2}].
+proof strict.
+  intros=> A.
+  fun. inline RO_H1.LRO.init.
+  swap {1} 9 7. swap {2} 9 7.
+  seq 6 6:
+    (={pks,b',i} /\
+     AKE.mSk{1} = G0_1.mSk{2} /\
+     AKE.cSession{1} = G0_1.cSession{1}).
+(*     AKE.cH1{1} = G0_1.cH1{2} /\
+     AKE.cH2{1} = G0_1.cH2{2} /\
+   (*  AKE.mH1{1} = RO_H1.LRO.m{2} /\ *)
+     AKE.sH1{1} = G0_1.sH1{2} /\
+     AKE.mH2{1} = G0_1.mH2{2} /\
+     AKE.sH2{1} = G0_1.sH2{2} /\
+     AKE.mStarted{1} = G0_1.mStarted{2} /\
+     AKE.mCompleted{1} =  G0_1.mCompleted{2} /\
+     AKE.evs{1} = G0_1.evs{2} /\
+     AKE.test{1} = G0_1.test{2}
+*)
+  eqobs_in. admit.
+
